Checkpoint

new/golang/defn/mem.v
@@ -21,10 +21,6 @@ Section defs.
 Context `{!NamedUnderlyingTypes}.
 Context `{ffi_syntax}.
 
-Definition alloc_def (V : Type) `{!IntoVal V} : val := (λ: <>, ref #(zero_val V)).
-Program Definition alloc := sealed @alloc_def.
-Definition alloc_unseal : alloc = _ := seal_eq _.
-
 Inductive is_primitive : go.type → Prop :=
 | is_primitive_uint64 : is_primitive uint64
 | is_primitive_uint32 : is_primitive uint32
@@ -44,15 +40,27 @@ Inductive is_primitive : go.type → Prop :=
 | is_primitive_map kt vt : is_primitive (go.MapType kt vt)
 | is_primitive_channel dir t : is_primitive (go.ChannelType dir t).
 
-Class MemOps :=
-{
-  load : go.type → val;
-  store : go.type → val;
-  size : go.type → Z;
+Inductive is_primitive_zero_val : go.type → ∀ {V} `{!IntoVal V}, V → Prop :=
+| is_primitive_zero_val_uint64 : is_primitive_zero_val uint64 (W64 0)
+| is_primitive_zero_val_uint32 : is_primitive_zero_val uint32 (W32 0)
+| is_primitive_zero_val_uint16 : is_primitive_zero_val uint16 (W16 0)
+| is_primitive_zero_val_uint8 : is_primitive_zero_val uint8 (W8 0)
+| is_primitive_zero_val_int64 : is_primitive_zero_val int64 (W64 0)
+| is_primitive_zero_val_int32 : is_primitive_zero_val int32 (W32 0)
+| is_primitive_zero_val_int16 : is_primitive_zero_val int16 (W16 0)
+| is_primitive_zero_val_int8 : is_primitive_zero_val int8 (W8 0).
 
-  is_load_underlying t : load t = load (to_underlying t);
-  is_load_primitive t (H : is_primitive t) : load t = (λ: "l", ! "l")%V;
-  is_load_struct fds :
+Global Arguments alloc {_ _} (t).
+Global Arguments load {_ _} (t).
+Global Arguments store {_ _} (t).
+Global Arguments goose_lang.size {_ _} (t).
+Existing Class GoContext.
+Class MemOps `{!GoContext} :=
+{
+  alloc_underlying t : alloc t = alloc (to_underlying t);
+  alloc_primitive t `{!IntoVal V} (v : V) (H : is_primitive_zero_val t v) :
+    alloc t = (λ: <>, ref #v)%V;
+  alloc_struct fds :
     let body := (foldl (λ '(offset, ld) (fd : go.field_decl),
                           (offset,
                              (ld, (match fd with
@@ -61,89 +69,49 @@ Class MemOps :=
                                    end)
                                     (BinOp (OffsetOp offset) #(W64 1) "l"))%E)
                    ) (0, Val #()) fds) in
+    alloc (go.StructType fds) = (λ: "l", body.2)%V;
+
+  load_underlying t : load t = load (to_underlying t);
+  load_primitive t (H : is_primitive t) : load t = (λ: "l", ! "l")%V;
+  load_struct fds :
+    let body := (foldl (λ '(offset, ld) (fd : go.field_decl),
+                          (offset,
+                             (ld, (match fd with
+                                   | go.FieldDecl _ t 
+                                   | go.EmbeddedField _ t => load t
+                                   end)
+                                    (BinOp (OffsetOp offset) "l" #(W64 1)))%E)
+                   ) (0, Val #()) fds) in
     load (go.StructType fds) = (λ: "l", body.2)%V;
-  is_load_array n elem :
+  load_array n elem :
     let body := (Z.iter n
                    (λ '(offset, ld),
                       (offset + 1,
                          (ld, load elem
-                                (BinOp (OffsetOp (offset * size elem))
-                                   #(W64 1) "l"))%E)
+                                (BinOp (OffsetOp (offset * goose_lang.size elem))
+                                  "l" #(W64 1)))%E)
                    ) (0, Val #())) in
     load (go.ArrayType n elem) = (λ: "l", body.2)%V;
 
-  size_underlying t : size t = size (to_underlying t);
-  size_primitive t (H : is_primitive t) : size t = 1;
-  size_struct fds : size (go.StructType fds) =
+  size_underlying t : goose_lang.size t = goose_lang.size (to_underlying t);
+  size_primitive t (H : is_primitive t) : goose_lang.size t = 1;
+  size_struct fds : goose_lang.size (go.StructType fds) =
                     foldl Z.add 0 ((λ fd, match fd with
                                           | go.FieldDecl _ t
-                                          | go.EmbeddedField _ t => size t
+                                          | go.EmbeddedField _ t => goose_lang.size t
                                           end
                                    ) <$> fds);
-  size_array n elem : size (go.ArrayType n elem) = n * size elem;
+  size_array n elem : goose_lang.size (go.ArrayType n elem) = n * goose_lang.size elem;
 }.
 
-Context `{!MemOps}.
-
-Record foo_t := 
-  mk {
-      a : w64;
-    }.
-Global Instance into_val_foo : IntoVal foo_t :=
-  {| to_val_def := λ v, (#v.(a), #())%V; zero_val := (mk (zero_val _)) |}.
-
-Definition foo : go.type := go.Named "foo"%go [].
-Definition foo_impl : go.type := go.StructType [(go.FieldDecl "a"%go uint64)].
-
-Class foo_type_assumptions : Prop :=
-  {
-    foo_underlying : named_to_underlying "foo"%go [] = foo_impl
-  }.
-
-Context `{!foo_type_assumptions}.
-
-Goal size (go.ArrayType 3 foo) = 3.
-  rewrite size_array size_underlying /= foo_underlying
-    size_struct /= size_primitive //. constructor.
-Qed.
-
-Definition struct_field_get (field_name : go_string) (t : go.type) : val :=
-  match to_underlying t with
-  | go.StructType fds =>
-      (* Look for the first field named `field_name`. *)
-      
-  end
-.
-
-Goal load (go.ArrayType 3 foo) = (λ: "l", ! "l")%V.
-  rewrite is_load_array /=. vm_compute Z.add.
-  rewrite is_load_underlying /=. foo_underlying.
-  rewrite is_load_struct /=.
-
-Goal load foo = (λ: "l", ! "l")%V.
-  rewrite is_load_underlying /= foo_underlying.
-  rewrite is_load_struct /=.
-
-  rewrite is_load_primitive; [|constructor].
-
-
-(* load t -> (load f1, load f2, load f3) when underlying(t) is a struct with
-   fields f1, f2, f3. *)
-Inductive is_load : go.type → val → Prop :=
-| is_load_uint64 t (H : is_primitive t) : is_load t (λ: "l", "l")%V
-| is_load_struct t fds (H : underlying t = go.StructType fds)
-                 (field_loads : list val)
-  :
-  is_load t (λ: "l", "l")%V
-.
-
+(*
 Definition load_def (t : go.type) : val := mem.load (to_mem_type t).
 Program Definition load := sealed @load_def.
 Definition load_unseal : load = _ := seal_eq _.
 
 Definition store_def (t : go.type) : val := mem.store (to_mem_type t).
 Program Definition store := sealed @store_def.
-Definition store_unseal : store = _ := seal_eq _.
+Definition store_unseal : store = _ := seal_eq _. *)
 
 End defs.
 End go.
